libcrux-ml-kem/src/vector.rs
@@ -143,7 +143,7 @@ fn montgomery_multiply_by_constant(mut v: PortableVector, c: i16) -> PortableVec
 ///
 /// The NIST FIPS 203 standard can be found at
 /// <https://csrc.nist.gov/pubs/fips/203/ipd>.
-#[cfg_attr(hax, hax_lib::requires(fe < (crate::constants::FIELD_MODULUS as u16)))]
+#[cfg_attr(hax, hax_lib::requires(fe < (FIELD_MODULUS as u16)))]
 #[cfg_attr(hax, hax_lib::ensures(|result|
         hax_lib::implies(833 <= fe && fe <= 2596, || result == 1) &&
         hax_lib::implies(!(833 <= fe && fe <= 2596), || result == 0)
@@ -179,7 +179,7 @@ pub(crate) fn compress_message_coefficient(fe: u16) -> u8 {
          coefficient_bits == 5 ||
          coefficient_bits == 10 ||
          coefficient_bits == 11) &&
-         fe < (crate::constants::FIELD_MODULUS as u16)))]
+         fe < (FIELD_MODULUS as u16)))]
 #[cfg_attr(hax,
      hax_lib::ensures(
      |result| result >= 0 && result < 2i16.pow(coefficient_bits as u32)))]
